Triangluar
==========


# Trigonometric【三角函数】



![Triangular](tfdef.png)

$\begin{align}\sin\theta=\frac{b}{c},\quad\csc\theta=\frac{c}{b}\end{align}$

$\begin{align}\cos\theta=\frac{a}{c},\quad\sec\theta=\frac{c}{a}\end{align}$

$\begin{align}\tan\theta=\frac{b}{a},\quad\cot\theta=\frac{a}{b}\end{align}$



#### Pythagoras Theorem 【勾股定理】

$a^2+b^2=c^2$

$\left\{\begin{array}{l}a=m^2-n^2\\b=2mn&,m>n>0\\c=m^2+n^2\end{array}\right.$



#### Cosine Theorem【余弦定理】

For any triangle in the Euclidean plane with sides $a,b,c$ and opposite angles $A,B,C$, respectively.

$c^2=a^2+b^2-2ab\cos C$



#### Sine Theorem【正弦定理】

For any triangle in the Euclidean plane with sides $a,b,c$ and opposite angles $A,B,C$, respectively, the equalities

$\begin{aligned}\frac{a}{\sin A}=\frac{b}{\sin B}=\frac{c}{\sin C}=2R\end{aligned}$

hold, where $R$ is the radius of the circumscribed circle.




#### Double angle formula【倍角公式】

$\sin^2\theta+\cos^2\theta=1$

$\begin{aligned}\sin\alpha+\cos\alpha=\sqrt{2}\sin(\alpha+\frac{\pi}{2})\end{aligned}$

$\sin2\alpha=2\sin\alpha\cos\alpha$

$\cos2\alpha=\cos^2\alpha-\sin^2\alpha=1-2\sin^2\alpha=2\cos^2\alpha-1$

$\begin{aligned}\tan2\alpha=\frac{2\tan\alpha}{\tan^2\alpha-1}\end{aligned}$



##### Half angles

$\begin{aligned}\sin\frac{\alpha}{2}=\pm\sqrt{\frac{1-\cos\alpha}{2}}\end{aligned}$

$\begin{aligned}\cos\frac{\alpha}{2}=\pm\sqrt{\frac{1+\cos\alpha}{2}}\end{aligned}$

$\begin{aligned}\tan\frac{\alpha}{2}=\pm\sqrt{\frac{1-\cos\alpha}{1+\cos\alpha}}=\frac{\sin\alpha}{1+\cos\alpha}=\frac{1-\cos\alpha}{\sin\alpha}\end{aligned}$

$\begin{aligned}\cot\frac{\alpha}{2}=\frac{1+\cos\alpha}{\sin\alpha}=\frac{\sin\alpha}{1-\cos\alpha}\end{aligned}$



##### Three times

$\begin{aligned}\sin3\alpha=3\sin\alpha-4\sin^3\alpha=4\sin\alpha\sin\left(\frac{\pi}{3}+\alpha\right)\sin\left(\frac{\pi}{3}-\alpha\right)\end{aligned}$

$\begin{aligned}\cos3\alpha=4\cos^3\alpha-3\cos\alpha=4\cos\alpha\cos\left(\frac{\pi}{3}+\alpha\right)\cos\left(\frac{\pi}{3}-\alpha\right)\end{aligned}$

$\begin{aligned}\tan3\alpha=\frac{\tan^3\alpha-3\tan\alpha}{3\tan^2\alpha-1}=\tan\alpha\tan\left(\frac{\pi}{3}+\alpha\right)\tan\left(\frac{\pi}{3}-\alpha\right)\end{aligned}$

$\begin{aligned}\cot3\alpha=\frac{\cot^3\alpha-3\cot\alpha}{3\cot^2\alpha-1}\end{aligned}$

$\begin{aligned}\sec3\alpha=\frac{\sec^3\alpha}{4-3\sec^2\alpha}\end{aligned}$

$\begin{aligned}\csc3\alpha=\frac{\csc^3\alpha}{3\csc^2\alpha-4}\end{aligned}$




##### Four times

$\begin{aligned}\sin4\alpha=-4\cos\alpha\sin\alpha\left(2\sin^2\alpha-1\right)\end{aligned}$

$\begin{aligned}\cos4\alpha=1-8\cos^4\alpha+8\cos^4\alpha\end{aligned}$

$\begin{aligned}\tan4\alpha=\frac{4\tan\alpha-4\tan^3\alpha}{1-6\tan^2\alpha+\tan^4\alpha}\end{aligned}$



##### Five times

$\begin{aligned}\sin5\alpha=16\sin^5\alpha-20\sin^3\alpha+5\sin\alpha\end{aligned}$

$\begin{aligned}\cos5\alpha=16\cos^5\alpha-20\cos^3\alpha+5\cos\alpha\end{aligned}$

$\begin{aligned}\tan5\alpha=\tan\alpha\frac{5-10\tan^2\alpha+\tan^4\alpha}{1-10\tan^2\alpha+5\tan^4\alpha}\end{aligned}$




##### Six times

$\begin{aligned}\sin6\alpha=2\cos\alpha\sin\alpha(2\sin\alpha+1)(2\sin\alpha-1)(4\sin^2\alpha-3)\end{aligned}$

$\begin{aligned}\cos6\alpha=(2\cos^2\alpha-1)(16\cos^4\alpha-16\cos\alpha+1)\end{aligned}$

$\begin{aligned}\tan6\alpha=\frac{-6\tan\alpha+20\tan^3\alpha-6\tan^5\alpha}{\tan^6\alpha-15\tan^4\alpha+15\tan^2\alpha-1}\end{aligned}$



##### Seven times

$\begin{aligned}\sin7\alpha=-\sin\alpha\left(56\sin^2\alpha-112\sin^4\alpha-64\sin^6\alpha-7\right)\end{aligned}$

$\begin{aligned}\cos7\alpha=\cos\alpha\left(56\cos^2\alpha-112\cos^4\alpha-64\cos^6\alpha-7\right)\end{aligned}$

$\begin{aligned}\tan7\alpha=\tan\alpha\frac{\tan^6\alpha-21\tan^4\alpha+35\tan^2\alpha-7}{7\tan^6\alpha-35\tan^4\alpha+21\tan^2\alpha-1}\end{aligned}$



##### De Moivre's formula 【棣莫弗定理】

$(\cos\theta+i\sin\theta)^n=\cos n\theta+i\sin n\theta$






$(\sin\alpha+\sin\beta)(\sin\alpha-\sin\beta)=\sin(\alpha+\beta)\sin(\alpha-\beta)$

$\begin{aligned}\cos^n\theta=\frac{1}{2^n}\sum^n_{k=0}{\rm C}^k_n\cos(2k-n)\theta\end{aligned}$

$\begin{aligned}\sin^n\theta=\frac{1}{2^n}\sum^n_{k=0}(-1)^k{\rm{C}}^k_n\cos\left((2k-n)\theta+\frac{n\pi}{2}\right)\end{aligned}$




#### Prosthaphaeresis【积化和差】

$\begin{aligned}\sin\alpha\cos\beta=\frac{1}{2}\Big[\sin(\alpha+\beta)+\sin(\alpha-\beta)\Big]\end{aligned}$

$\begin{aligned}\sin\alpha\sin\beta=\frac{1}{2}\Big[\cos(\alpha-\beta)-\cos(\alpha+\beta)\Big]\end{aligned}$

$\begin{aligned}\cos\alpha\cos\beta=\frac{1}{2}\Big[\cos(\alpha+\beta)+\cos(\alpha-\beta)\Big]\end{aligned}$



#### Sum-to-product Identities Fomulas【和差化积】

$\begin{aligned}\sin\alpha+\sin\beta=2\sin\frac{\alpha+\beta}{2}\cos\frac{\alpha-\beta}{2}\end{aligned}$

$\begin{aligned}\cos\alpha+\cos\beta=2\cos\frac{\alpha+\beta}{2}\cos\frac{\alpha-\beta}{2}\end{aligned}$

$\begin{aligned}\cos\alpha-\cos\beta=2\sin\frac{\alpha+\beta}{2}\sin\frac{\alpha-\beta}{2}\end{aligned}$




#### 常见角度的三角函数

| $\theta$ | $\sin\theta$ | $\cos\theta$ | $\tan\theta$ | $\cot\theta$ | $\sec\theta$ | $\csc\theta$ |
| -------- | ------------ | ------------ | ------------ | ------------ | ------------ | ------------ |
| $15^{\circ}\quad\frac{\pi}{12}$ | $\frac{\sqrt{6}-\sqrt{2}}{4}$ | $\frac{\sqrt{6} +\sqrt{2}}{4}$ | $2-\sqrt{3}$ | $2+\sqrt{3}$ | $\sqrt{6}-\sqrt{2}$ | $\sqrt{6}+\sqrt{2}$ |
| $18^{\circ}\quad\frac{\pi}{10}$ | $\frac{\sqrt{5}-1}{4}$ | $\frac{\sqrt{10+2\sqrt{5}}}{4}$ | $\frac{\sqrt{25-10\sqrt{5}}}{5}$ | $\sqrt{5+2\sqrt{5}}$ | $\frac{\sqrt{50-10\sqrt{5}}}{5}$ | $\sqrt{5}+1$ |
| $22.5^{\circ}\quad\frac{\pi}{8}$ | $\frac{\sqrt{2-\sqrt{2}}}{2}$ | $\frac{\sqrt{2+\sqrt{2}}}{2}$ | $\sqrt{2}-1$ | $\sqrt{2}+1$ | $\sqrt{4-2\sqrt{2}}$ | $\sqrt{4+2\sqrt{2}}$ |
| $30^{\circ}\quad\frac{\pi}{6}$ | $\frac{1}{2}$ | $\frac{\sqrt{3}}{2}$ | $\frac{\sqrt{3}}{3}$ | $\sqrt{3}$ | $\frac{2\sqrt{3}}{3}$ | $2$ |
| $36^{\circ}\quad\frac{\pi}{5}$ | $\frac{\sqrt{10-2\sqrt{5}}}{4}$ | $\frac{\sqrt{5}+1}{4}$ | $\sqrt{5-2\sqrt{5}}$ |  $\frac{\sqrt{25+10\sqrt{5}}}{5}$ | $\sqrt{5}-1$ | $\frac{\sqrt{50+10\sqrt{5}}}{5}$ |
| $45^{\circ}\quad\frac{\pi}{4}$ | $\frac{\sqrt{2}}{2}$ | $\frac{\sqrt{2}}{2}$ | $1$ | $1$ | $\sqrt{2}$ | $\sqrt{2}$ |
| $54^{\circ}\quad\frac{3\pi}{10}$ | $\frac{\sqrt{5}+1}{4}$ | $\frac{\sqrt{10-2\sqrt{5}}}{4}$ | $\frac{\sqrt{25+10\sqrt{5}}}{5}$ | $\sqrt{5-2\sqrt{5}}$ | $\frac{50+10\sqrt{5}}{5}$ | $\sqrt{5}-1$ |
| $60^{\circ}\quad\frac{\pi}{3}$ | $\frac{\sqrt{3}}{2}$ | $\frac{1}{2}$ | $\sqrt{3}$ | $\frac{\sqrt{3}}{3}$ | $2$ | $\frac{2\sqrt{3}}{3}$ |
| $67.5^{\circ}\quad\frac{3\pi}{8}$ | $\frac{\sqrt{2+\sqrt{2}}}{2}$ | $\frac{\sqrt{2-\sqrt{2}}}{2}$ | $\sqrt{2}+1$ | $\sqrt{2}-1$ | $\sqrt{4+2\sqrt{2}}$ | $\sqrt{4-2\sqrt{2}}$ |
| $72^{\circ}\quad\frac{2\pi}{5}$ | $\frac{\sqrt{10+2\sqrt{5}}}{4}$ | $\frac{\sqrt{5}-1}{4}$ | $\sqrt{5+2\sqrt{5}}$ | $\frac{\sqrt{25-10\sqrt{5}}}{5}$ | $\sqrt{5}+1$ | $\frac{\sqrt{50-10\sqrt{5}}}{5}$ |
| $75^{\circ}\quad\frac{5\pi}{12}$ | $\frac{\sqrt{6}+\sqrt{2}}{4}$ | $\frac{\sqrt{6}-\sqrt{2}}{4}$ | $2+\sqrt{3}$ | $2-\sqrt{3}$ | $\sqrt{6}+\sqrt{2}$ | $\sqrt{6}-\sqrt{2}$ |
| $90^{\circ}\quad\frac{\pi}{2}$ | $1$ | $0$ | $\to\infty$ | $0$ | $\to\infty$ | $1$ |
| $180^{\circ}\quad\pi$ | $0$ | $-1$ | $0$ | $\to\infty$ | $-1$ | $\to\infty$ |
| $270^{\circ}\quad\frac{3\pi}{2}$ | $-1$ | $0$ | $\to\infty$ | $0$ | $\to\infty$ | $-1$ |
| $360^{\circ}\quad 2\pi$ | $0$ | $1$ | $0$ | $\to\infty$ | $1$ | $\to\infty$ |






## Hyperbolic Function【双曲函数】

$\begin{align}\sinh x=\frac{e^{x}-e^{-x}}{2}=-i\sin ix\end{align}$

$\begin{align}\cosh x=\frac{e^{x}+e^{-x}}{2}=\cos ix\end{align}$

$\begin{align}\tanh x=\frac{e^x-e^{-x}}{e^x+e^{-x}}=-i \tan ix\end{align}$

$\begin{align}\coth x=\frac{e^x+e^{-x}}{e^x-e^{-x}}=i\cot ix\end{align}$

$\begin{align}sech x=\frac{2}{e^{x}+e^{-x}}=\sec ix\end{align}$

$\begin{align}csch x=\frac{2}{e^{x}-e^{-x}}=i\csc ix\end{align}$


# 三角函数关系索引
* $e^{ix}=\cos x+i\sin x$
* $e^{i\pi}+1=0$


* $\sin^2\theta+\cos^2\theta=1$
* $\begin{align}\tan\theta=\frac{\sin\theta}{\cos\theta}\end{align}$
* $\begin{align}\cot\theta=\frac{\cos\theta}{\sin\theta}\end{align}$
* $\begin{align}\cos^2\theta=\frac{1}{1+\tan^2\theta}\end{align}$
* $\begin{align}\sin^2\theta=\frac{1}{1+\cot^2\theta}\end{align}$

* $\sin(\alpha\pm\beta)=\sin\alpha\cos\beta\pm\cos\alpha\sin\beta$
* $\cos(\alpha\pm\beta)=\cos\alpha\cos\beta\mp\sin\alpha\sin\beta$
* $\begin{align}\tan(\alpha\pm\beta)=\frac{\tan\alpha\pm\tan\beta}{1\mp\tan\alpha\tan\beta}\end{align}$

* $\begin{align}\sin\alpha\sin\beta=\frac{1}{2}\Big[\cos(\alpha-\beta)+\cos(\alpha+\beta)\Big]\end{align}$
* $\begin{align}\cos\alpha\cos\beta=\frac{1}{2}\Big[\cos(\alpha-\beta)-\cos(\alpha+\beta)\Big]\end{align}$
* $\begin{align}\sin\alpha\cos\beta=\frac{1}{2}\Big[\sin(\alpha-\beta)+\sin(\alpha+\beta)\Big]\end{align}$
* $\begin{align}\cos\alpha\sin\beta=\frac{1}{2}\Big[\sin(\alpha+\beta)-\sin(\alpha-\beta)\Big]\end{align}$

* $\begin{align}\sin\alpha+\sin\beta=2\sin\frac{\alpha+\beta}{2}\cos\frac{\alpha-\beta}{2}\end{align}$
* $\begin{align}\sin\alpha-\sin\beta=2\cos\frac{\alpha+\beta}{2}\sin\frac{\alpha-\beta}{2}\end{align}$
* $\begin{align}\cos\alpha+\cos\beta=2\cos\frac{\alpha+\beta}{2}\cos\frac{\alpha-\beta}{2}\end{align}$
* $\begin{align}\cos\alpha-\cos\beta=-2\sin\frac{\alpha+\beta}{2}\sin\frac{\alpha-\beta}{2}\end{align}$

* $\begin{align}\tan\alpha+\tan\beta=\frac{\sin(\alpha+\beta)}{\cos\alpha\cos\beta}\end{align}$
* $\begin{align}\tan\alpha-\tan\beta=\frac{\sin(\alpha-\beta)}{\cos\alpha\cos\beta}\end{align}$
* $\begin{align}\cot\alpha+\cot\beta=\frac{\sin(\alpha+\beta)}{\sin\alpha\sin\beta}\end{align}$
* $\begin{align}\cot\alpha-\cot\beta=-\frac{\sin(\alpha-\beta)}{\sin\alpha\sin\beta}\end{align}$
* $\begin{align}\tan\alpha+\cot\beta=\frac{\cos(\alpha-\beta)}{\cos\alpha\sin\beta}\end{align}$
* $\begin{align}\tan\alpha-\cot\beta=-\frac{\cos(\alpha+\beta)}{\cos\alpha\sin\beta}\end{align}$

* $\begin{align}\sin^2\alpha-\sin^2\beta=\sin(\alpha+\beta)\sin(\alpha-\beta)\end{align}$
* $\begin{align}\cos^2\alpha-\cos^2\beta=-\sin(\alpha+\beta)\sin(\alpha-\beta)\end{align}$
* $\begin{align}\cos^2\alpha-\sin^2\beta=\cos(\alpha+\beta)\cos(\alpha-\beta)\end{align}$
* $\begin{align}\sin^2\alpha-\cos^2\beta=-\cos(\alpha+\beta)\cos(\alpha-\beta)\end{align}$

